More development

Equipotence.v
@@ -5,7 +5,8 @@ Definition inverse f :=
   (fun p => exists u, exists v, p ≅ tuple v u /\ tuple u v ∈ f).
 
 Record injection_def (x y : V) (f : V) := {
-  injection_def_fun : function_def x y f;
+  injection_def_def : forall u, u ∈ x -> exists v, v ∈ y /\ tuple u v ∈ f;
+  injection_def_fun : forall u v1 v2, tuple u v1 ∈ f -> tuple u v2 ∈ f -> v1 ≅ v2;
   injection_def_inj : forall u1 u2 v, tuple u1 v ∈ f -> tuple u2 v ∈ f -> u1 ≅ u2
 }.
 
@@ -15,6 +16,16 @@ Record bijection_def (x y : V) (f : V) := {
   bijection_def_funl : forall u v1 v2, tuple u v1 ∈ f -> tuple u v2 ∈ f -> v1 ≅ v2;
   bijection_def_funr : forall u1 u2 v, tuple u1 v ∈ f -> tuple u2 v ∈ f -> u1 ≅ u2
 }.
+
+Instance Proper_injection_def : Proper (V_eq ==> V_eq ==> V_eq ==> iff) injection_def.
+Proof.
+assert (HP : Proper (V_eq ==> V_eq ==> V_eq ==> Basics.impl) injection_def).
+{ intros x1 x2 Hx y1 y2 Hy f1 f2 Hf [H1 H2 H3]; split; intros.
+  + destruct (H1 u); [rewrite Hx; assumption|]; eexists; rewrite <- Hy, <- Hf; eassumption.
+  + eapply H2; rewrite Hf; eassumption.
+  + eapply H3; rewrite Hf; eassumption. }
+repeat intro; split; apply HP; solve [assumption|symmetry; assumption].
+Qed.
 
 Definition injection x y := comprehension (powerset (product x y)) (injection_def x y).
 Definition bijection x y := comprehension (powerset (product x y)) (bijection_def x y).
@@ -28,14 +39,35 @@ assert (HP : Proper (V_eq ==> iff) (fun p => exists u, exists v, p ≅ tuple v u
 split; intros H.
 + apply comprehension_spec; [assumption|].
   split; [|exists x, y; split; [reflexivity|assumption]].
-  apply product_spec; exists y, x; split; [|split; [|reflexivity]].
-  - apply comprehension_spec.
-    admit.
-Admitted.
+  assert (Hmx : singleton x ∈ union f).
+  { apply union_spec; exists (tuple x y); split; [|assumption].
+    apply pair_spec; left; reflexivity. }
+  assert (Hmy : pair x y ∈ union f).
+  { apply union_spec; exists (tuple x y); split; [|assumption].
+    apply pair_spec; right; reflexivity. }
+  assert (Hdx : x ∈ domain f).
+  { apply comprehension_spec.
+    + intros ? ? ?; repeat f_equiv; assumption.
+    + split; [|assumption].
+      apply union_spec; exists (singleton x).
+      split; [apply singleton_spec; reflexivity|assumption]. }
+  assert (Hdy : y ∈ codomain f).
+  { apply comprehension_spec.
+    + intros ? ? ?; repeat f_equiv; intros ?; repeat f_equiv; assumption.
+    + split; [|exists x; intuition].
+      apply union_spec; exists (pair x y).
+      split; [|assumption]; apply pair_spec; right; reflexivity. }
+  apply product_spec; exists y, x; now intuition.
++ apply comprehension_spec in H; [|do 3 intro; do 2 (f_equiv; intro); repeat f_equiv; assumption].
+  destruct H as [Hl [u [v [Heq Hf]]]].
+  assert (Hrw := tuple_inj_l _ _ _ _ Heq); rewrite <- Hrw in Hf; clear Hrw.
+  assert (Hrw := tuple_inj_r _ _ _ _ Heq); rewrite <- Hrw in Hf; clear Hrw.
+  assumption.
+Qed.
 
 Lemma injection_function : forall x y f, injection_def x y f -> function_def x y f.
 Proof.
-intros x y f [? ?]; assumption.
+intros x y f [? ? H]; split; assumption.
 Qed.
 
 Lemma injection_bijection : forall x y f,
@@ -47,11 +79,4 @@ assert (HP : Proper (V_eq ==> iff) (fun p => exists u, exists v, p ≅ tuple v u
   exists u, v; rewrite <- Hx; assumption. }
 split; intros H.
 + destruct H as [Hdefl Hdefr Hfunl Hfunr]; split; split.
-  - split; assumption.
-  - assumption.
-  - split.
-    { intros v Hv; destruct (Hdefr v Hv) as [u [Hu Hf]].
-      exists u; split; [assumption|].
-      apply comprehension_spec; [assumption|].
-      split; [|exists u, v; now intuition].
 Admitted.
