CC_model.v
@@ -1,0 +1,175 @@
+Require PTS_type_eq.
+Require Import Morphisms Base Cartesian.
+
+Module Sorts <: PTS_base.term_sig.
+
+Inductive sorts := set | kind.
+
+Definition Sorts := sorts.
+
+End Sorts.
+
+Module Axioms <: PTS_base.pts_sig (Sorts).
+
+Import Sorts.
+
+Inductive ax : sorts -> sorts -> Prop :=
+  ax_constr : ax set kind.
+
+Definition Ax := ax.
+
+Inductive rel : sorts -> sorts -> sorts -> Prop :=
+| rel_lam : rel set set set
+| rel_F : rel kind set set
+| rel_dep : rel set kind kind
+| rel_ho : rel kind kind kind.
+
+Definition Rel := rel.
+
+End Axioms.
+
+Declare Module Term : PTS_term.ut_term_mod Sorts.
+Declare Module Env : PTS_env.ut_env_mod Sorts Term.
+Declare Module Red : PTS_red.ut_red_mod Sorts Term.
+Declare Module SR : PTS_sr.ut_sr_mod Sorts Axioms Term Env Red.
+Declare Module CC : PTS_type_eq.ut_typ_eq_mod Sorts Axioms Term Env Red SR.
+
+Import Sorts Axioms.
+
+(* Record function_def (x y f : V) : Prop :={
+  function_def_def : forall u : V, u ∈ x -> ;
+}. *)
+
+Definition app f x :=
+  comprehension (union (union f)) (fun α => tuple x α ∈ f).
+
+Definition reify (A : V) (f : V -> V) : V :=
+  comprehension (product A (union (collection A f)))
+  (fun p => exists x, exists α, α ∈ f x /\ p ≅ tuple x α).
+
+Definition dsum (A : V) (B : V) : V :=
+  comprehension (product A (union (union B)))
+  (fun p => exists x, exists y, x ∈ A /\ y ∈ app B x /\ p ≅ tuple x y).
+
+Definition dprd (A : V) (B : V) : V :=
+  comprehension (powerset (dsum A B))
+  (fun f => function_def A (collection A (app B)) f).
+
+Instance Proper_app : Proper (V_eq ==> V_eq ==> V_eq) app.
+Proof.
+intros x1 x2 Hx y1 y2 Hy; unfold app; f_equiv.
++ rewrite Hx; reflexivity.
++ intros z1 z2 Hz; rewrite Hx, Hy, Hz; reflexivity.
+Qed.
+
+Instance Proper_reify : Proper (V_eq ==> (V_eq ==> V_eq) ==> V_eq) reify.
+Proof.
+intros x1 x2 Hx f1 f2 Hf; unfold reify; f_equiv.
++ f_equiv; [assumption|].
+  f_equiv; f_equiv; [assumption|assumption].
++ intros y1 y2 Hy; f_equiv; intros x; f_equiv; intros α; f_equiv.
+  - f_equiv; apply Hf; reflexivity.
+  - split; rewrite Hy; tauto.
+Qed.
+
+Lemma dsum_spec : forall A B p,
+  p ∈ dsum A B <-> (exists x, exists y, x ∈ A /\ y ∈ app B x /\ p ≅ tuple x y).
+Proof.
+intros A B p.
+assert (HP : Proper (V_eq ==> iff) (fun p0 : V => exists x y : V, x ∈ A /\ y ∈ app B x /\ p0 ≅ tuple x y)).
+{ intros x1 x2 Hx; f_equiv; intros x; f_equiv; intros y.
+  do 2 f_equiv; split; rewrite Hx; trivial. }
+split; intros H.
++ apply comprehension_spec in H; [|assumption].
+  destruct H as [Hp [x [y [Hx [Hy Heq]]]]].
+  exists x, y; intuition.
++ destruct H as [x [y [Hx [Hy Heq]]]].
+  apply comprehension_spec; [assumption|].
+  split; [|exists x, y; split; [|split]; first [assumption|reflexivity]].
+  apply product_spec; exists x, y.
+  split; [assumption|]; split; [|assumption]; clear p Heq.
+  apply comprehension_spec in Hy; [|intros z1 z2 Hz; rewrite Hz; reflexivity].
+  now intuition.
+Qed.
+
+Lemma reify_spec : forall A f x, Proper (V_eq ==> V_eq) f ->
+  x ∈ A -> app (reify A f) x ≅ f x.
+Proof.
+intros A f x Hf Hx.
+assert (HP : Proper (V_eq ==> iff) (fun p : V => exists x α : V, α ∈ f x /\ p ≅ tuple x α)).
+{ clear - Hf; intros p1 p2 Hp; f_equiv; intros x; f_equiv; intros α.
+  f_equiv; split; rewrite Hp; tauto. }
+apply extensionality; apply included_spec; intros z Hz.
++ apply comprehension_spec in Hz.
+  - destruct Hz as [Hz Hi].
+    apply union_spec in Hz; destruct Hz as [r [Hz Hr]].
+    apply union_spec in Hr; destruct Hr as [s [Hr Hs]].
+    apply comprehension_spec in Hi; [|assumption].
+    destruct Hi as [Hi [u [α [Hp Ht]]]].
+    assert (Hrw := tuple_inj_l _ _ _ _ Ht); rewrite Hrw in *; clear x Hrw.
+    assert (Hrw := tuple_inj_r _ _ _ _ Ht); rewrite Hrw in *; assumption.
+  - clear - Hf; intros x1 x2 Hx; rewrite Hx; reflexivity.
++ apply comprehension_spec.
+  - clear - Hf; intros x1 x2 Hx; rewrite Hx; reflexivity.
+  - assert (Hm : tuple x z ∈ reify A f).
+    { apply comprehension_spec; [exact HP|].
+      split; [|exists x, z; split; [assumption|reflexivity]].
+      apply product_spec; exists x, z.
+      split; [assumption|]; split; [|reflexivity].
+      apply union_spec; exists (f x); split; [assumption|].
+      apply collection_spec; [exact Hf|].
+      exists x; split; [assumption|reflexivity]. }
+    split; [|assumption].
+    apply union_spec; exists (pair x z).
+    split; [apply pair_spec; right; reflexivity|].
+    apply union_spec; exists (tuple x z).
+    split; [apply pair_spec; right; reflexivity|].
+    assumption.
+Qed.
+
+Lemma reify_impredicative : forall A, reify A (fun _ => empty) ≅ empty.
+Proof.
+intros A; apply extensionality; apply included_spec; intros x Hx.
++ exfalso; apply comprehension_spec in Hx.
+  - destruct Hx as [Hx [p [α [Hα Hp]]]].
+    apply empty_spec in Hα; contradiction.
+  - clear; intros x1 x2 Hx; f_equiv; intros x; f_equiv; intros α.
+    split; rewrite Hx; auto.
++ apply empty_spec in Hx; contradiction.
+Qed.
+
+Lemma app_empty : forall x, app empty x ≅ empty.
+Proof.
+intros x.
+pose (Hrw := reify_impredicative (singleton x)).
+rewrite <- Hrw at 1; rewrite reify_spec.
++ reflexivity.
++ intros _ _ _; reflexivity.
++ apply singleton_spec; reflexivity.
+Qed.
+
+Program Fixpoint term_eval (Γ : Env.Env) (M : Term.Term) {struct M} : V :=
+match M with
+| Term.Var n => empty
+| Term.Sort set => powerset (singleton empty)
+| Term.Sort kind => empty
+| Term.App M N => app (term_eval Γ M) (term_eval Γ N)
+| Term.Pi A B => dprd (term_eval Γ A) (term_eval (cons A Γ) B)
+| Term.La A M => reify (term_eval Γ A) (fun x => term_eval (cons A Γ) M)
+end.
+
+Lemma term_eval_type_eq_compat : forall Γ M1 M2 A, CC.typ_eq Γ M1 M2 A ->
+  term_eval Γ M1 ≅ term_eval Γ M2
+with term_eval_type_compat : forall Γ M A, CC.typ Γ M A ->
+  term_eval Γ M ∈ term_eval Γ A.
+Proof.
+{ intros Γ M1 M2 A HR; induction HR; simpl; try solve [f_equiv; assumption].
+  + admit.
+  + f_equiv; [assumption|]; intros _ _ _.
+    admit.
+  + symmetry; assumption.
+  + etransitivity; eassumption.
+  + assumption.
+  + rewrite reify_spec; [|intros _ _ _; reflexivity|].
+    admit.
+Admitted.
